Improve terminology, add more definitions about partitions

TheoremsAboutAlgorithms/Partitions.lean
@@ -13,6 +13,7 @@ import Init.Data.Fin.Basic
 -- Terminology:
 --   * For any n : ℕ, a Cell n is a set of Fin n, i.e. a subset of the base set {0, 1, ..., n - 1}.
 --   * For any n : ℕ, a Split n is a set of Cell n, i.e. a collection of subsets of the base set {0, 1, ..., n - 1}.
+--     Note that these don't have to be disjoint, so this is not the same as a partition of the base set.
 --
 -- By using Fin n to represent the base set, we can use the definition Setoid.IsPartition from the standard library
 -- to talk about partitions, which seems to present a nicer api than the one we would get by using Set ℕ and using
@@ -26,16 +27,20 @@ abbrev Split (n : ℕ) := Set (Cell n)
 --                                                  Cells                                                             --
 ------------------------------------------------------------------------------------------------------------------------
 
+-- TODO: Maybe there's a more elegant way to use all those mapped functions
+def Cell.cast {n m : ℕ} (h : n = m) (cell : Cell n) : Cell m
+  := Fin.cast h '' cell
+
 def Cell.castSucc {n : ℕ} (cell : Cell n) : Cell (n + 1)
   := Fin.castSucc '' cell
 
--- TODO: Use a more descriptive name for this (and namespace it).
+-- TODO: Maybe we can find a better name yet (it's alright, but not totally satisfactory).
 -- This is essentially cell ↦ {n} ∪ cell
-def Cell.transform {n : ℕ} (cell : Cell n) : Cell (n + 1)
+def Cell.insertSuccMax {n : ℕ} (cell : Cell n) : Cell (n + 1)
   := cell.castSucc.insert (Fin.ofNat n)
 
 -- TODO: Look for a nicer proof of this.
-theorem Cell.transform_is_disjoint_insert {n : ℕ} (cell : Cell n)
+theorem Cell.insertSuccMax_is_disjoint_insert {n : ℕ} (cell : Cell n)
   : Disjoint {Fin.ofNat n} cell.castSucc := by
     apply disjoint_iff.mpr
     simp [Cell.castSucc, Fin.castSucc, Fin.ofNat]
@@ -48,39 +53,46 @@ theorem Cell.transform_is_disjoint_insert {n : ℕ} (cell : Cell n)
 --                                                  Splits                                                            --
 ------------------------------------------------------------------------------------------------------------------------
 
+def Split.cast {n m : ℕ} (h : n = m) (split : Split n) : Split m
+  := Cell.cast h '' split
+
 def Split.castSucc {n : ℕ} (split : Split n) : Split (n + 1)
   := Cell.castSucc '' split
 
-def Split.removeCellAndCastSucc {n : ℕ} (split : Split n) (cell : Cell n) : Split (n + 1)
-  := Split.castSucc (split \ singleton cell)
+def Split.removeCell {n : ℕ} (split : Split n) (cell : Cell n) : Split n
+  := split \ singleton cell
 
--- TODO: Use a more descriptive name for this (and namespace it).
+-- TODO: Maybe we can find a better name yet (it's alright, but not totally satisfactory).
 -- We don't require targetCell ∈ split, because we want to be able to have ∅ as a target cell as well.
 -- This is essentially split ↦ {targetCell.transform} ∪ (split \ {targetCell})
-def transformSplit {n : ℕ} (split : Split n) (targetCell : Cell n) : Split (n + 1)
-  := (Split.removeCellAndCastSucc split targetCell).insert targetCell.transform
+def Split.insertSuccMaxAt {n : ℕ} (split : Split n) (targetCell : Cell n) : Split (n + 1)
+  := (split.removeCell targetCell).castSucc.insert targetCell.insertSuccMax
 
-theorem transformSplit_is_disjoint_insert {n : ℕ} (split : Split n) (targetCell : Cell n)
-  : Disjoint {targetCell.transform} (Split.removeCellAndCastSucc split targetCell) := by
+theorem Split.insertSuccMaxAt_is_disjoint_insert {n : ℕ} (split : Split n) (targetCell : Cell n)
+  : Disjoint {targetCell.insertSuccMax} (split.removeCell targetCell).castSucc := by
     apply disjoint_iff.mpr
-    simp [Split.removeCellAndCastSucc, Fin.castSucc, Split.castSucc]
+    simp [Split.removeCell, Split.castSucc, Fin.castSucc]
     intro cell _ _
-    have h_k : ¬ (∀ (x : Fin (n + 1)), x ∈ cell.castSucc ↔ x ∈ targetCell.transform) := by
+    have h_k : ¬ (∀ (x : Fin (n + 1)), x ∈ cell.castSucc ↔ x ∈ targetCell.insertSuccMax) := by
       simp [not_iff]
       exists (Fin.ofNat n)
       constructor
       · intro
-        simp [Cell.transform]
+        simp [Cell.insertSuccMax]
         exact Set.mem_insert _ _
       · intro
         apply Set.disjoint_singleton_left.mp
-        exact Cell.transform_is_disjoint_insert cell
-    have := Set.ext_iff (s := cell.castSucc) (t := targetCell.transform)
+        exact Cell.insertSuccMax_is_disjoint_insert cell
+    have := Set.ext_iff (s := cell.castSucc) (t := targetCell.insertSuccMax)
     exact (not_congr this).mpr h_k
 
--- TODO: Find a better name for this (and namespace it).
-def toSplitsWithN {n : ℕ} (split : Split n) : Set (Split (n + 1))
-  := {transformSplit split cell | cell ∈ split.insert ∅}
+-- TODO: Maybe we can find a better name yet (it's alright, but not totally satisfactory).
+-- TODO: Do we even need this if we have the version below?
+def Split.insertSuccMax {n : ℕ} (split : Split n) : Set (Split (n + 1))
+  := {split.insertSuccMaxAt cell | cell ∈ split.insert ∅}
+
+def Split.insertSuccMax' {n : ℕ} (h : n > 0) (split : Split (n - 1)) : Set (Split n)
+  := Split.cast (Nat.sub_add_cancel h) '' split.insertSuccMax
 
 ------------------------------------------------------------------------------------------------------------------------
 --                                              Partitions                                                            --
@@ -90,14 +102,16 @@ def Split.IsPartition {n : ℕ} (split : Split n) : Prop
   := Setoid.IsPartition split
 
 def partitions (n : ℕ) : Set (Split n)
-  := {split | Split.IsPartition split}
+  := {split | split.IsPartition}
 
-notation "ℙ[" n "]" => partitions n
+abbrev ℙ (n : ℕ) := partitions n
 
 def recursivePartitions (n : ℕ) : Set (Split n)
-  -- TODO: Needs helper function wrapping (toSplitsWithN split) in the appropriate Fin.cast to get
-  --       Fin (n - 1 + 1) = Fin n in the types.
-  --:= ⋃ partition ∈ ℙ[n - 1], toSplitsWithN partition
-  := sorry
+  := match n with
+    | 0 => ∅
+    | m + 1 => ⋃ partition ∈ ℙ m, partition.insertSuccMax' (Nat.succ_pos m)
 
-notation "ℙᵣ[" n "]" => recursivePartitions n
+abbrev ℙᵣ (n : ℕ) := recursivePartitions n
+
+theorem partitions_eq_recursivePartitions (n : ℕ) : ℙ n = ℙᵣ n := by
+  sorry
